state (without proving yet) fold_two_spec, which folds over the same
map with two different functions and different initial values.

It seems that everything map.fold related we need follows from that,
in particular these are proven:
- the original map.fold_spec
- fold_spec_with_order, which says that the iteration order of map.fold
  only depends on the map, but not on f and the intial value
- map.fold_comm
- map.fold_remove
- map.fold_put

compiler/src/compiler/PipelineWithRename.v
@@ -76,11 +76,126 @@ Section WithWordAndMem.
   Qed.
 End WithWordAndMem.
 
+Require Import Coq.Sorting.Permutation.
+
 (* TODO move to coqutil *)
+Module List.
+  Section WithA.
+    Context {A: Type} {a_eqb: A -> A -> bool} {a_eqb_spec: EqDecider a_eqb}.
+
+    Lemma fold_right_change_order{R: Type}(f: A -> R -> R)
+          (f_comm: forall a1 a2 r, f a1 (f a2 r) = f a2 (f a1 r)):
+      forall l1 l2: list A,
+        Permutation l1 l2 ->
+        forall r0, fold_right f r0 l1 = fold_right f r0 l2.
+    Proof.
+      induction 1; intros.
+      - reflexivity.
+      - simpl. f_equal. auto.
+      - simpl. apply f_comm.
+      - rewrite IHPermutation1, IHPermutation2. reflexivity.
+    Qed.
+  End WithA.
+End List.
+
 Module map.
   Section WithMap.
     Context {key value} {map : map.map key value} {ok : map.ok map}.
     Context {key_eqb: key -> key -> bool} {key_eq_dec: EqDecider key_eqb}.
+
+    Definition tuples(m: map): list (key * value) :=
+      map.fold (fun l k v => (k, v) :: l) nil m.
+
+    Axiom fold_two_spec:
+      forall {R1 R2: Type} (P: map -> R1 -> R2 -> Prop)
+             (f1: R1 -> key -> value -> R1) (f2: R2 -> key -> value -> R2) r01 r02,
+        P map.empty r01 r02 ->
+        (forall k v m r1 r2, map.get m k = None ->
+                             P m r1 r2 ->
+                             P (map.put m k v) (f1 r1 k v) (f2 r2 k v)) ->
+        forall m, P m (map.fold f1 r01 m) (map.fold f2 r02 m).
+
+    Lemma fold_spec:
+      forall {R: Type} (P: map -> R -> Prop) (f: R -> key -> value -> R) r0,
+        P map.empty r0  ->
+        (forall k v m r, map.get m k = None -> P m r -> P (map.put m k v) (f r k v)) ->
+        forall m, P m (map.fold f r0 m).
+    Proof.
+      intros.
+      eapply fold_two_spec with (f1 := f) (f2 := f) (r01 := r0) (r02 := r0) (m0 := m); eauto.
+    Qed.
+
+    Lemma tuples_NoDup: forall m, NoDup (tuples m).
+    Proof.
+      intros.
+      eapply proj1 with (B := forall k v, List.In (k, v) (tuples m) -> map.get m k = Some v).
+      unfold tuples.
+      eapply map.fold_spec.
+      - simpl. intuition constructor.
+      - intros. destruct H0. intuition (try constructor; try assumption).
+        + intro C. specialize H1 with (1 := C). congruence.
+        + simpl in *. destruct H2.
+          * inversion H2; rewrite map.get_put_same; congruence.
+          * rewrite map.get_put_dec.
+            destr (key_eqb k k0).
+            -- subst k0. specialize H1 with (1 := H2). congruence.
+            -- eauto.
+    Qed.
+
+    Lemma fold_to_tuples_fold : forall {R: Type} (f: R -> key -> value -> R) r0 m,
+        map.fold f r0 m =
+        List.fold_right (fun '(k, v) r => f r k v) r0 (tuples m).
+    Proof.
+      intros. unfold tuples.
+      eapply fold_two_spec with
+          (f1 := f)
+          (f2 := (fun (l : list (key * value)) (k : key) (v : value) => (k, v) :: l)).
+      - reflexivity.
+      - intros. subst. simpl. reflexivity.
+    Qed.
+
+    Lemma tuples_spec: forall (m: map) (k : key) (v : value),
+        In (k, v) (tuples m) <-> map.get m k = Some v.
+    Proof.
+      intro m. unfold tuples.
+      eapply map.fold_spec; intros; split; intros; simpl in *.
+      - contradiction.
+      - rewrite map.get_empty in H. discriminate.
+      - rewrite map.get_put_dec.
+        destr (key_eqb k k0).
+        + subst k0. destruct H1.
+          * inversion H1; subst v0. reflexivity.
+          * specialize (H0 k v0). apply proj1 in H0. specialize (H0 H1).
+            congruence.
+        + destruct H1.
+          * congruence.
+          * eapply H0. assumption.
+      - rewrite map.get_put_dec in H1.
+        destr (key_eqb k k0).
+        + subst k0. inversion H1; subst v0. auto.
+        + right. eapply H0. assumption.
+    Qed.
+
+    Lemma fold_spec_with_order : forall m, exists (l: list (key * value)),
+      (forall k v, List.In (k, v) l <-> map.get m k = Some v) /\
+      forall {R: Type} (f: R -> key -> value -> R) r0,
+        map.fold f r0 m = List.fold_right (fun '(k, v) r => f r k v) r0 l.
+    Proof.
+      intros. eexists. split.
+      - eapply tuples_spec.
+      - intros. eapply fold_to_tuples_fold.
+    Qed.
+
+    Lemma fold_comm{R: Type}(f: R -> key -> value -> R)
+          (f_comm: forall r k1 v1 k2 v2, f (f r k1 v1) k2 v2 = f (f r k2 v2) k1 v1):
+      forall r0 m k v,
+        map.fold f (f r0 k v) m = f (map.fold f r0 m) k v.
+    Proof.
+      intros.
+      eapply fold_two_spec with (f1 := f) (f2 := f) (r01 := f r0 k v) (r02 := r0).
+      - reflexivity.
+      - intros. subst. apply f_comm.
+    Qed.
 
     Lemma map_ind(P: map -> Prop):
       P map.empty ->
@@ -93,32 +208,40 @@ Module map.
       eapply Step; assumption.
     Qed.
 
+    Lemma tuples_put: forall m k v,
+        map.get m k = None ->
+        forall k0 v0, List.In (k0, v0) (tuples (map.put m k v)) <-> List.In (k0, v0) ((k, v) :: tuples m).
+    Proof.
+      intros.
+      rewrite (tuples_spec (map.put m k v)).
+      simpl.
+      rewrite (tuples_spec m).
+      rewrite map.get_put_dec.
+      destr (key_eqb k k0); intuition congruence.
+    Qed.
+
     Lemma fold_put{R: Type}(f: R -> key -> value -> R)
           (f_comm: forall r k1 v1 k2 v2, f (f r k1 v1) k2 v2 = f (f r k2 v2) k1 v1):
       forall r0 m k v,
         map.get m k = None ->
         map.fold f r0 (map.put m k v) = f (map.fold f r0 m) k v.
     Proof.
-      intros r0 m. pattern m.
-      eapply map_ind; intros.
-      - rewrite map.fold_empty. rewrite map.fold_singleton. reflexivity.
-      - rewrite map.get_put_dec in H1.
-        destr (key_eqb k k0). 1: discriminate.
-        rewrite H by assumption.
-    Abort.
-
-    Lemma fold_last{R: Type}(f: R -> key -> value -> R):
-      forall r0 m,
-        (m = map.empty) \/
-        (exists k v r, map.fold f r0 m = f r k v).
-    Proof.
-      intros r0 m.
-      eapply map.fold_spec; intros.
-      - auto.
-      - right. destruct H0.
-        + subst. eauto.
-        + destruct H0 as [ k1 [v1 [ r1 IH ] ] ].
-          subst. eauto.
+      intros.
+      do 2 rewrite fold_to_tuples_fold.
+      match goal with
+      | |- ?L = f (fold_right ?F r0 (tuples m)) k v =>
+        change (L = fold_right F r0 ((k, v) :: tuples m))
+      end.
+      apply List.fold_right_change_order.
+      - intros [k1 v1] [k2 v2] r. apply f_comm.
+      - apply NoDup_Permutation.
+        + apply tuples_NoDup.
+        + constructor.
+          * pose proof (tuples_spec m k v). intuition congruence.
+          * apply tuples_NoDup.
+        + intros [k0 v0].
+          rewrite (tuples_put m k v H).
+          reflexivity.
     Qed.
 
     Lemma fold_remove{R: Type}(f: R -> key -> value -> R)
@@ -127,45 +250,14 @@ Module map.
         map.get m k = Some v ->
         map.fold f r0 m = f (map.fold f r0 (map.remove m k)) k v.
     Proof.
-      intros r0 m. pattern m.
-      eapply map_ind; intros.
-      - rewrite map.get_empty in H. discriminate.
-      - rewrite map.get_put_dec in H1.
-        destr (key_eqb k k0).
-        + apply Option.eq_of_eq_Some in H1.
-          subst v0 k0.
-    Abort.
-
-    Lemma fold_pull{R: Type}(f: R -> key -> value -> R)
-          (f_comm: forall r k1 v1 k2 v2, f (f r k1 v1) k2 v2 = f (f r k2 v2) k1 v1):
-      forall r0 m k v,
-        map.fold f (f r0 k v) m = f (map.fold f r0 m) k v.
-    Proof.
-      intros r0 m. pattern m.
-      eapply map_ind; intros.
-      - rewrite !map.fold_empty. reflexivity.
-      -
-    Abort.
-
-    Lemma fold_put{R: Type}(f: R -> key -> value -> R)
-          (f_comm: forall r k1 v1 k2 v2, f (f r k1 v1) k2 v2 = f (f r k2 v2) k1 v1):
-      forall r0 m k v,
-        map.get m k = None ->
-        map.fold f r0 (map.put m k v) = f (map.fold f r0 m) k v.
-    Proof.
       intros.
-      erewrite (map.fold_remove f f_comm r0 (map.put m k v) k v).
-      2: apply map.get_put_same.
-      replace (map.remove (map.put m k v) k) with m.
-      1: reflexivity.
-      apply map.map_ext.
-      intros.
-      rewrite map.get_remove_dec.
-      destr (key_eqb k k0).
-      1: congruence.
-      rewrite map.get_put_diff; congruence.
+      replace m with (map.put (map.remove m k) k v) at 1.
+      - rewrite fold_put; eauto using map.get_remove_same.
+      - apply map.map_ext.
+        intros.
+        rewrite map.get_put_dec.
+        destr (key_eqb k k0); try rewrite map.get_remove_diff; congruence.
     Qed.
-
   End WithMap.
 End map.
 
